Lift fuel resources to joint models

fairneris/fair_resources.v
@@ -1,12 +1,12 @@
 From iris.algebra Require Import auth gmap gset excl.
 From iris.proofmode Require Import tactics.
-From fairneris Require Import fairness fuel map_included_utils.
+From fairneris Require Import fairness fuel map_included_utils env_model.
 
-Canonical Structure ModelO (Mdl : FairModel) := leibnizO Mdl.
-Canonical Structure RoleO (Mdl : FairModel) := leibnizO (Mdl.(fmrole)).
+Canonical Structure ModelO `{GoodLang Λ} (Mdl : UserModel Λ) := leibnizO Mdl.
+Canonical Structure RoleO `{GoodLang Λ} (Mdl : UserModel Λ) := leibnizO (Mdl.(usr_role)).
 Canonical Structure localeO (Λ : language) := leibnizO (locale Λ).
 
-Class fairnessGpreS `{Countable (locale Λ)} `(LM: LiveModel Λ M) Σ := {
+Class fairnessGpreS `{GoodLang Λ} `(LM: LiveModel Λ (joint_model M Net)) Σ := {
   fairnessGpreS_model :> inG Σ (authUR (optionUR (exclR (ModelO M))));
   fairnessGpreS_model_fuel_mapping :>
     inG Σ (authUR (gmapUR (localeO Λ)
@@ -14,7 +14,7 @@ Class fairnessGpreS `{Countable (locale Λ)} `(LM: LiveModel Λ M) Σ := {
   fairnessGpreS_model_free_roles :> inG Σ (authUR (gset_disjUR (RoleO M)));
 }.
 
-Class fairnessGS `{Countable (locale Λ)} `(LM : LiveModel Λ M) Σ := FairnessGS {
+Class fairnessGS `{GoodLang Λ} `(LM : LiveModel Λ (joint_model M Net)) Σ := FairnessGS {
   fairness_inG :> fairnessGpreS LM Σ;
   (** Underlying model *)
   fairness_model_name : gname;
@@ -24,19 +24,47 @@ Class fairnessGS `{Countable (locale Λ)} `(LM : LiveModel Λ M) Σ := FairnessG
   fairness_model_free_roles_name : gname;
 }.
 
-Global Arguments fairnessGS {_ _ _ _} LM Σ.
-Global Arguments fairness_model_name {_ _ _ _ LM Σ} _.
-Global Arguments fairness_model_fuel_mapping_name {Λ _ _ M LM Σ} _ : assert.
-Global Arguments fairness_model_free_roles_name {Λ _ _ M LM Σ} _ : assert.
+Global Arguments fairnessGS {_ _ _ _ _ _ _ _ _ _ _ _} LM Σ.
+Global Arguments fairness_model_name {_ _ _ _ _ _ _ _ _ _ _ _ LM Σ} _.
+Global Arguments fairness_model_fuel_mapping_name {Λ _ _ _ _ _ _ _ _ _ M Net LM Σ} _ : assert.
+Global Arguments fairness_model_free_roles_name {Λ _ _ _ _ _ _ _ _ _ M Net LM Σ} _ : assert.
 
-Definition fairnessΣ Λ M `{Countable (locale Λ)} : gFunctors := #[
+Definition fairnessΣ Λ `{GoodLang Λ} M : gFunctors := #[
    GFunctor (authUR (optionUR (exclR (ModelO M))));
    GFunctor (authUR (gmapUR (localeO Λ)
                             (exclR $ gmapUR (RoleO M) natO)));
    GFunctor (authUR (gset_disjUR (RoleO M)))
 ].
 
-Global Instance subG_fairnessGpreS {Σ} `{Countable (locale Λ)} `{LM : LiveModel Λ M}
+(* We need more parameters than the iris tactic supports... *)
+Ltac solve_inG :=
+  intros;
+   lazymatch goal with
+   | H:subG (?xΣ _ _ _ _ _ _ _ _ _ _ _ _) _ |- _ => try unfold xΣ in H
+   | H:subG (?xΣ _ _ _ _ _ _ _ _ _ _ _) _ |- _ => try unfold xΣ in H
+   | H:subG (?xΣ _ _ _ _ _ _ _ _ _ _) _ |- _ => try unfold xΣ in H
+   | H:subG (?xΣ _ _ _ _ _ _ _ _ _) _ |- _ => try unfold xΣ in H
+   | H:subG (?xΣ _ _ _ _ _ _ _ _) _ |- _ => try unfold xΣ in H
+   | H:subG (?xΣ _ _ _ _ _ _ _) _ |- _ => try unfold xΣ in H
+   | H:subG (?xΣ _ _ _ _ _ _) _ |- _ => try unfold xΣ in H
+   | H:subG (?xΣ _ _ _ _ _) _ |- _ => try unfold xΣ in H
+   | H:subG (?xΣ _ _ _ _) _ |- _ => try unfold xΣ in H
+   | H:subG (?xΣ _ _ _) _ |- _ => try unfold xΣ in H
+   | H:subG (?xΣ _ _) _ |- _ => try unfold xΣ in H
+   | H:subG (?xΣ _) _ |- _ => try unfold xΣ in H
+   | H:subG ?xΣ _ |- _ => try unfold xΣ in H
+   end;
+  repeat match goal with
+    | H:subG (gFunctors.app _ _) _ |- _ => apply subG_inv in H; destruct H
+  end;
+  repeat match goal with
+    | H:subG _ _ |- _ => move : (H) ; apply subG_inG in H || clear H
+  end;
+  intros; simpl in *; try assumption; split; assumption || by apply _.
+
+
+
+Global Instance subG_fairnessGpreS {Σ} `{GoodLang Λ} `{LM : LiveModel Λ (joint_model M Net)}
        :
   subG (fairnessΣ Λ M) Σ -> fairnessGpreS LM Σ.
 Proof. solve_inG. Qed.
@@ -163,13 +191,13 @@ Section map_imap.
 End map_imap.
 
 Section model_state_interp.
-  Context `{Countable (locale Λ)}.
-  Context `{LM: LiveModel Λ M}.
+  Context `{GoodLang Λ}.
+  Context `{LM: LiveModel Λ (joint_model M Net)}.
   Context {Σ : gFunctors}.
   Context {fG: fairnessGS LM Σ}.
   Context `{!invGS_gen HasNoLc Σ}.
 
-  Notation Role := (M.(fmrole)).
+  Notation Role := (usr_role M).
 
   Definition auth_fuel_mapping_is
              (m: gmap (locale Λ) (gmap Role nat)) : iProp Σ :=
@@ -215,21 +243,20 @@ Section model_state_interp.
              (fuel_map : gmap (locale Λ) (gmap Role nat)) :=
      ∀ ζ, ζ ∉ locales_of_list tp → fuel_map !! ζ = None.
 
-  Definition config_update_state : iProp Σ :=
-    ∀ m1 m2 cl fl, ⌜ LM.(lm_cfg_action) m1 cl = (fl, m2) ⌝ -∗ auth_model_is m1 ={⊤}=∗ auth_model_is m2.
+  Definition usr_state (δ : LiveStateData Λ (joint_model M Net)) : M := δ.(ls_under).1.
+  Definition env_state (δ : LiveStateData Λ (joint_model M Net)) : Net := δ.(ls_under).2.
 
-  Definition model_state_interp (tp: list $ expr Λ) (δ: LiveStateData Λ M): iProp Σ :=
-    □ config_update_state ∗
+  Definition model_state_interp (tp: list $ expr Λ) (δ: LiveStateData Λ (joint_model M Net)): iProp Σ :=
     ∃ fuel_map,
       ⌜ fuel_map_le fuel_map δ.(ls_map) ⌝ ∗
-      ⌜ fuel_map_preserve_dead fuel_map (M.(live_roles) δ) ⌝ ∗
+      ⌜ fuel_map_preserve_dead fuel_map (M.(usr_live_roles) (usr_state δ)) ⌝ ∗
       ⌜ fuel_map_preserve_threadpool tp fuel_map ⌝ ∗
-      auth_model_is δ ∗ auth_fuel_mapping_is fuel_map.
+      auth_model_is (usr_state δ) ∗ auth_fuel_mapping_is fuel_map.
 
   Lemma model_state_interp_tids_smaller (δ : LiveState _ _) tp :
     model_state_interp tp δ -∗ ⌜ tids_smaller tp δ ⌝.
   Proof.
-    iIntros "(?&%m&[_ %Heq]&%&%Hbig&_)".
+    iIntros "(%m&[_ %Heq]&%&%Hbig&_)".
     iPureIntro.
     intros ζ Hin.
     assert (¬ (ζ ∉ locales_of_list tp)).
@@ -250,12 +277,13 @@ Lemma own_proper `{inG Σ X} γ (x y: X):
 Proof. intros ->. naive_solver. Qed.
 
 Section model_state_lemmas.
-  Context `{Countable (locale Λ)}.
-  Context `{LM: LiveModel Λ M}.
+  Context `{GoodLang Λ}.
+  Context `{LM: LiveModel Λ (joint_model M Net)}.
   Context {Σ : gFunctors}.
+  Context `{EqDecision (expr Λ)}.
   Context {fG: fairnessGS LM Σ}.
 
-  Notation Role := (M.(fmrole)).
+  Notation Role := (M.(usr_role)).
 
   Definition has_fuels (ζ: locale Λ) (fs: gmap Role nat) : iProp Σ :=
     frag_fuel_mapping_is {[ ζ := fs ]}.
@@ -303,8 +331,8 @@ Notation "tid ↦M R" := (has_fuels tid R) (at level 20, format "tid  ↦M  R") 
 Notation "tid ↦M++ R" := (has_fuels_S tid R) (at level 20, format "tid  ↦M++  R") : bi_scope.
 
 Section adequacy.
-  Context `{Countable (locale Λ)}.
-  Context `{LM: LiveModel Λ M}.
+  Context `{GoodLang Λ}.
+  Context `{LM: LiveModel Λ (joint_model M Net)}.
   Context {Σ : gFunctors}.
   Context {fG: fairnessGpreS LM Σ}.
 
@@ -319,8 +347,8 @@ Section adequacy.
   Qed.
 
   Definition init_fuel_map (s0: M) (ζ0: locale Λ) :
-    gmap (locale Λ) (exclR $ gmap (fmrole M) nat) :=
-    {[ ζ0 := Excl (gset_to_gmap (LM.(lm_fl) s0) (M.(live_roles) s0)) ]}.
+    gmap (locale Λ) (exclR $ gmap (usr_role M) nat) :=
+    {[ ζ0 := Excl (gset_to_gmap (usr_fl s0) (usr_live_roles s0)) ]}.
 
   Lemma model_fuel_mapping_init (s0: M) (ζ0: locale Λ) :
     ⊢ |==> ∃ γ,
@@ -344,12 +372,12 @@ Section adequacy.
 End adequacy.
 
 Section model_state_lemmas.
-  Context `{Countable (locale Λ)}.
-  Context `{LM: LiveModel Λ M}.
-  Context `{EqDecision (expr Λ)}.
+  Context `{GoodLang Λ}.
+  Context `{LM: LiveModel Λ (joint_model M Net)}.
   Context {Σ : gFunctors}.
   Context {fG: fairnessGS LM Σ}.
   Context `{!invGS_gen HasNoLc Σ}.
+  Context `{EqDecision (expr Λ)}.
 
   Lemma update_model δ δ1 δ2:
     auth_model_is δ1 -∗ frag_model_is δ2 ==∗ auth_model_is δ ∗ frag_model_is δ.
@@ -369,14 +397,14 @@ Section model_state_lemmas.
   Qed.
 
   Lemma model_agree' δ1 s2 n:
-    model_state_interp n δ1 -∗ frag_model_is s2 -∗ ⌜ ls_under δ1 = s2 ⌝.
+    model_state_interp n δ1 -∗ frag_model_is s2 -∗ ⌜ (ls_under δ1).1 = s2 ⌝.
   Proof.
-    iIntros "Hsi Hs2". iDestruct "Hsi" as "(?&%fm&?&_&_&Hs1&_)".
+    iIntros "Hsi Hs2". iDestruct "Hsi" as "(%fm&?&_&_&Hs1&_)".
     iApply (model_agree with "Hs1 Hs2").
   Qed.
 
-  Lemma has_fuels_agree (ζ : locale Λ) (fs : gmap (fmrole M) nat)
-        (m : gmap (locale Λ) (gmap (fmrole M) nat)) :
+  Lemma has_fuels_agree (ζ : locale Λ) (fs : gmap (usr_role M) nat)
+        (m : gmap (locale Λ) (gmap (usr_role M) nat)) :
     auth_fuel_mapping_is m -∗ has_fuels ζ fs -∗ ⌜m !! ζ = Some fs⌝.
   Proof.
     iIntros "Hauth Hfrag".
@@ -407,7 +435,6 @@ Section model_state_lemmas.
     auth_fuel_mapping_is (<[ζ := fs']>fm) ∗ has_fuels ζ fs'.
   Proof.
     iIntros "Hfm Hfs".
-    rewrite /has_fuels_S.
     iDestruct (has_fuels_agree with "Hfm Hfs") as %Hagree.
     iMod (own_update_2 with "Hfm Hfs") as "[$ $]"; [|done].
     apply auth_update.
@@ -420,8 +447,8 @@ Section model_state_lemmas.
     - eapply exclusive_local_update. done.
   Qed.
 
-  Lemma has_fuels_decr (ζ : locale Λ) (fs : gmap (fmrole M) nat)
-        (m : gmap (locale Λ) (gmap (fmrole M) nat)) :
+  Lemma has_fuels_decr (ζ : locale Λ) (fs : gmap (usr_role M) nat)
+        (m : gmap (locale Λ) (gmap (usr_role M) nat)) :
     auth_fuel_mapping_is m -∗ has_fuels_S ζ fs ==∗
     auth_fuel_mapping_is (<[ζ := fs]>m) ∗ has_fuels ζ fs.
   Proof.
@@ -444,12 +471,12 @@ Section model_state_lemmas.
     model_state_interp tp δ -∗ has_fuels_S tid fs ==∗
     model_state_interp tp δ ∗ has_fuels tid fs.
   Proof.
-    iDestruct 1 as "(?&%fm&[%Hfmle%Hdom]&%Hfmdead&%Htp&Hδ & Hfm)".
+    iDestruct 1 as "(%fm&[%Hfmle%Hdom]&%Hfmdead&%Htp&Hδ & Hfm)".
     iIntros "Hfs".
     iDestruct (has_fuels_agree with "Hfm Hfs") as %Hagree.
     iMod (has_fuels_decr with "Hfm Hfs") as "[Hfm Hfs]".
     iModIntro. iFrame "Hfs".
-    iSplit. iFrame. iExists _. iFrame.
+    iExists _. iFrame.
     iPureIntro. repeat split.
     - eapply map_included_transitivity; [|done].
       rewrite -{2}(insert_id fm tid (S <$> fs)); [|done].
@@ -471,7 +498,7 @@ Section model_state_lemmas.
   Qed.
 
   Lemma model_state_interp_has_fuels_dealloc tid fs ρ tp δ δ' :
-    ρ ∉ live_roles _ δ →
+    ρ ∉ usr_live_roles δ →
     model_state_interp tp δ' -∗
     frag_model_is δ -∗
     has_fuels tid fs ==∗
@@ -482,7 +509,7 @@ Section model_state_lemmas.
     { assert (delete ρ fs = fs) as ->.
       { apply delete_notin. by rewrite -not_elem_of_dom. }
       by iIntros "$$$". }
-    iDestruct 1 as "(?&%fm&[%Hfmle%Hdom]&%Hfmdead&%Htp&Hm&Hfm)".
+    iDestruct 1 as "(%fm&[%Hfmle%Hdom]&%Hfmdead&%Htp&Hm&Hfm)".
     iIntros "Hst Hfs".
     iDestruct (model_agree with "Hm Hst") as %Heq. rewrite !Heq.
     assert (is_Some (fs !! ρ)) as [f HSome].
@@ -490,7 +517,7 @@ Section model_state_lemmas.
     iDestruct (has_fuels_agree with "Hfm Hfs") as %Hagree.
     iMod (has_fuels_delete with "Hfm Hfs") as "[Hfm Hfs]".
     iModIntro.
-    iFrame "Hst". iFrame "Hfs". iSplit; first iFrame.
+    iFrame "Hst". iFrame "Hfs".
     iExists _. iFrame. rewrite Heq. iFrame.
     iPureIntro.
     repeat split; try done.
@@ -527,12 +554,12 @@ Section model_state_lemmas.
   Qed.
 
   (* TODO: Move this *)
-  Lemma silent_step_suff_data_weak act fl `(δ: LiveState Λ M)
+  Lemma silent_step_suff_data_weak act fl `(δ: LiveState Λ (joint_model M Net))
         (fs fs' : gmap _ nat) ζ:
     δ.(ls_map) !! ζ = Some fs →
     fs ≠ ∅ →
     map_included (<) fs' fs →
-    (dom fs ∖ dom fs') ∩ M.(live_roles) δ = ∅ →
+    (dom fs ∖ dom fs') ∩ usr_live_roles (usr_state δ) = ∅ →
     ∃ δ', δ'.(ls_data) =
           {| ls_under := δ;
             ls_map := <[ζ := fs']> δ.(ls_map) |} ∧
@@ -540,20 +567,20 @@ Section model_state_lemmas.
   Proof.
     intros.
     apply (silent_step_suff_data fl δ fs fs' ∅ ζ None); try done.
-    - rewrite map_included_spec in H2. done.
+    - rewrite -> map_included_spec in *. done.
     - set_solver.
     - set_solver.
   Qed.
 
   (* TODO: Change original lemma to not existentially quantify new state *)
-  Lemma silent_step_suff_data_weak_alt act fl (δ δ' : LiveState Λ M)
+  Lemma silent_step_suff_data_weak_alt act fl (δ δ' : LiveState Λ (joint_model M Net))
         (fs fs' : gmap _ nat) ζ :
     δ.(ls_under) = δ'.(ls_under) →
     δ.(ls_map) !! ζ = Some fs →
     δ'.(ls_map) = <[ζ := fs']>δ.(ls_map) →
     fs ≠ ∅ →
     map_included (<) fs' fs →
-    (dom fs ∖ dom fs') ∩ M.(live_roles) δ = ∅ →
+    (dom fs ∖ dom fs') ∩ usr_live_roles (usr_state δ) = ∅ →
     ls_trans fl δ (Silent_step ζ act) δ'.
   Proof.
     rewrite map_included_spec. intros Hδ Hfs Hfs' Hne Hle Hlive.
@@ -572,15 +599,15 @@ Section model_state_lemmas.
       δ2.(ls_map) = <[ζ := fs2]>δ1.(ls_map) ∧
       fs1 ≠ ∅ ∧
       map_included (<) fs2 fs1 ∧
-      (dom fs1 ∖ dom fs2) ∩ M.(live_roles) δ1 = ∅.
+      (dom fs1 ∖ dom fs2) ∩ usr_live_roles (usr_state δ1) = ∅.
 
-  Lemma model_can_fuel_step_trans act fl ζ (δ δ' : LiveState Λ M) :
+  Lemma model_can_fuel_step_trans act fl ζ (δ δ' : LiveState Λ _) :
     model_can_fuel_step δ ζ δ' → ls_trans fl δ (Silent_step ζ act) δ'.
   Proof.
     destruct 1 as (?&?&?&?&?&?&?&?). by eapply silent_step_suff_data_weak_alt.
   Qed.
 
-  Definition decr_fuel_map (fs : gmap (fmrole M) nat) : gmap (fmrole M) nat :=
+  Definition decr_fuel_map (fs : gmap (usr_role M) nat) : gmap (usr_role M) nat :=
     (λ f, f - 1) <$> fs.
 
   Lemma decr_fuel_map_included fs : map_included (≤) (decr_fuel_map fs) fs.
@@ -591,9 +618,9 @@ Section model_state_lemmas.
   Qed.
 
   Definition filter_fuel_map
-             δ (ρs : gset (fmrole M)) (fs : gmap (fmrole M) nat) :
-      gmap (fmrole M) nat :=
-    (filter (λ ρf, ρf.1 ∈ M.(live_roles) δ.(ls_under) ∨ ρf.1 ∈ ρs)) fs.
+             (δ: LiveState Λ (joint_model M Net)) (ρs : gset (usr_role M)) (fs : gmap (usr_role M) nat) :
+      gmap (usr_role M) nat :=
+    (filter (λ ρf, ρf.1 ∈ usr_live_roles (usr_state δ) ∨ ρf.1 ∈ ρs)) fs.
 
   Lemma filter_fuel_map_included δ ρs fs :
     map_included (≤) (filter_fuel_map δ ρs fs) fs.
@@ -602,14 +629,14 @@ Section model_state_lemmas.
     intros k v1 Hm.
     exists v1. split; [|lia].
     pose proof (map_filter_subseteq
-                  (λ ρf : fmrole M * nat, ρf.1 ∈ live_roles M δ ∨ ρf.1 ∈ ρs) fs)
+                  (λ ρf : usr_role M * nat, ρf.1 ∈ usr_live_roles (usr_state δ) ∨ ρf.1 ∈ ρs) fs)
       as Hle.
     rewrite map_subseteq_spec in Hle.
     by apply Hle.
   Qed.
 
   Definition model_update_locale_role_map
-          δ (ρs : gset (fmrole M)) : gmap (fmrole M) nat → gmap (fmrole M) nat :=
+          δ (ρs : gset (usr_role M)) : gmap (usr_role M) nat → gmap (usr_role M) nat :=
     decr_fuel_map ∘ filter_fuel_map δ ρs.
 
   Lemma model_update_locale_role_map_map_included δ ρs fs :
@@ -621,9 +648,9 @@ Section model_state_lemmas.
   Qed.
 
   Definition model_update_locale_fuel_map
-          δ (ζ : locale Λ) (ρs : gset (fmrole M))
-          (fm : gmap (locale Λ) (gmap (fmrole M) nat)) :
-      gmap (locale Λ) (gmap (fmrole M) nat) :=
+          δ (ζ : locale Λ) (ρs : gset (usr_role M))
+          (fm : gmap (locale Λ) (gmap (usr_role M) nat)) :
+      gmap (locale Λ) (gmap (usr_role M) nat) :=
     <[ζ:= model_update_locale_role_map δ ρs (fm !!! ζ)]>fm.
 
   Program Definition model_update_decr (ζ : locale Λ) (δ : LM) : LM :=
@@ -664,10 +691,11 @@ Section model_state_lemmas.
     rewrite lookup_total_alt in Hfs2'.
     destruct (ls_map δ !! ζ1) as [fs1''|] eqn:Hfs1''; last first.
     { apply map_included_subseteq_inv in Hle1.
-      apply map_disjoint_dom. set_solver. }
+      apply map_disjoint_dom.
+      rewrite Hfs1'' /= in Hfs1'. simplify_eq. set_solver. }
     destruct (ls_map δ !! ζ2) as [fs2''|] eqn:Hfs2''; last first.
     { apply map_included_subseteq_inv in Hle2.
-      apply map_disjoint_dom. set_solver. }
+      apply map_disjoint_dom. rewrite Hfs2'' in Hfs2'. set_solver. }
     simplify_eq; simpl in *.
     specialize (Hdisj ζ1 ζ2 fs1'' fs2'' Hneq Hfs1'' Hfs2'').
     apply map_disjoint_spec.
@@ -677,6 +705,7 @@ Section model_state_lemmas.
     apply Hle1 in HSome1' as (?&?&?).
     rewrite map_included_spec in Hle2.
     apply Hle2 in HSome2' as (?&?&?).
+    rewrite -> Hfs1'', Hfs2'' in *.
     by eapply Hdisj.
   Qed.
   Next Obligation.
@@ -693,13 +722,13 @@ Section model_state_lemmas.
   Qed.
 
   Program Definition model_update_filter
-          (ζ : locale Λ) (ρs : gset (fmrole M)) (δ : LM) : LM :=
+          (ζ : locale Λ) (ρs : gset (usr_role M)) (δ : LM) : LM :=
     {|
       ls_data :=
         {| ls_under := δ.(ls_under);
            ls_map :=
              alter (filter
-                       (λ ρf, ρf.1 ∈ M.(live_roles) δ.(ls_under) ∨ ρf.1 ∈ ρs))
+                       (λ ρf, ρf.1 ∈ usr_live_roles (usr_state δ) ∨ ρf.1 ∈ ρs))
                        ζ δ.(ls_map); |};
     |}.
   Next Obligation.
@@ -734,10 +763,10 @@ Section model_state_lemmas.
     rewrite lookup_total_alt in Hfs2'.
     destruct (ls_map δ !! ζ1) as [fs1''|] eqn:Hfs1''; last first.
     { apply map_included_subseteq_inv in Hle1.
-      apply map_disjoint_dom. set_solver. }
+      apply map_disjoint_dom. rewrite Hfs1'' in Hfs1'. set_solver. }
     destruct (ls_map δ !! ζ2) as [fs2''|] eqn:Hfs2''; last first.
     { apply map_included_subseteq_inv in Hle2.
-      apply map_disjoint_dom. set_solver. }
+      apply map_disjoint_dom. rewrite Hfs2'' in Hfs2'. set_solver. }
     simplify_eq; simpl in *.
     specialize (Hdisj ζ1 ζ2 fs1'' fs2'' Hneq Hfs1'' Hfs2'').
     apply map_disjoint_spec.
@@ -747,6 +776,7 @@ Section model_state_lemmas.
     apply Hle1 in HSome1' as (?&?&?).
     rewrite map_included_spec in Hle2.
     apply Hle2 in HSome2' as (?&?&?).
+    rewrite -> Hfs1'', Hfs2'' in *.
     by eapply Hdisj.
   Qed.
   Next Obligation.
@@ -768,7 +798,7 @@ Section model_state_lemmas.
   Qed.
 
   Definition model_update_locale_fuel
-             (δ : LM) (ζ : locale Λ) (ρs : gset (fmrole M)) : LM :=
+             (δ : LM) (ζ : locale Λ) (ρs : gset (usr_role M)) : LM :=
     model_update_decr ζ $ model_update_filter ζ ρs δ.
 
   Lemma model_update_locale_spec extr (auxtr : auxiliary_trace LM) ζ c2 ρs:
@@ -787,7 +817,7 @@ Section model_state_lemmas.
     econstructor=>//; first by apply model_can_fuel_step_trans.
   Qed.
 
-  Definition map_disj (m : gmap (locale Λ) (gmap (fmrole M) nat)) :=
+  Definition map_disj (m : gmap (locale Λ) (gmap (usr_role M) nat)) :=
     ∀ ζ ζ' fs fs', ζ ≠ ζ' → m !! ζ = Some fs → m !! ζ' = Some fs' → fs ##ₘ fs'.
 
   Lemma decr_succ_compose_id : (λ f : nat, f - 1) ∘ S = id.
@@ -799,7 +829,7 @@ Section model_state_lemmas.
       k1 ≠ k2 → m !! k1 = Some vs1 → m !! k2 = Some vs2 → vs1 ##ₘ vs2.
 
   Lemma fuel_map_le_disj ζ1 ζ2 fm fs1 fs2 ρ
-        (fuel_map : gmap (locale Λ) (gmap (fmrole M) nat)) :
+        (fuel_map : gmap (locale Λ) (gmap (usr_role M) nat)) :
     fuel_map_le_inner fm fuel_map → map_inner_disj fuel_map →
     fm !! ζ1 = Some fs1 → fm !! ζ2 = Some fs2 →
     ρ ∈ dom fs1 → ρ ∈ dom fs2 →
@@ -823,7 +853,7 @@ Section model_state_lemmas.
   Qed.
 
   Lemma fuel_map_le_disj' ζ1 ζ2 fm fs1 fs2 fs1' fs2' ρ
-        (fuel_map : gmap (locale Λ) (gmap (fmrole M) nat)) :
+        (fuel_map : gmap (locale Λ) (gmap (usr_role M) nat)) :
     fuel_map_le_inner fm fuel_map → map_inner_disj fuel_map →
     fm !! ζ1 = Some fs1 → fm !! ζ2 = Some fs2 →
     fuel_map !! ζ1 = Some fs1' → fuel_map !! ζ2 = Some fs2' →
@@ -841,7 +871,7 @@ Section model_state_lemmas.
   Qed.
 
   (* TODO: Clean up *)
-  Lemma fuel_map_le_live_roles fm fm' (lρs : gset (fmrole M)) ζ ρs ρs' ρ :
+  Lemma fuel_map_le_live_roles fm fm' (lρs : gset (usr_role M)) ζ ρs ρs' ρ :
     map_inner_disj fm' → fuel_map_le_inner fm fm' →
     fuel_map_preserve_dead fm lρs →
     fm !! ζ = Some ρs → fm' !! ζ = Some ρs' →
@@ -858,8 +888,8 @@ Section model_state_lemmas.
       - rewrite /fuel_map_le_inner map_included_spec. apply Hfmle.
       - by apply elem_of_dom.
       - rewrite map_included_spec in Hfs''.
-        apply elem_of_dom in Hv2' as [??].
-        apply Hfs'' in H1. destruct H1 as (?&?&?).
+        apply elem_of_dom in Hv2' as [? Hsome].
+        apply Hfs'' in Hsome. destruct Hsome as (?&?&?).
         by apply elem_of_dom. }
     set_solver.
   Qed.
@@ -869,7 +899,7 @@ Section model_state_lemmas.
     ⌜model_can_fuel_step δ ζ ((model_update_locale_fuel δ ζ) (dom fs))⌝.
   Proof.
     iIntros (Hfs) "Hm Hfs".
-    iDestruct "Hm" as "(?&%fm&[%Hfmle%Hdom]&%Hfmdead&%Htp&Hm&Hfm)".
+    iDestruct "Hm" as "(%fm&[%Hfmle%Hdom]&%Hfmdead&%Htp&Hm&Hfm)".
     rewrite /model_can_fuel_step.
     iDestruct (has_fuels_agree with "Hfm Hfs") as %Hagree.
     rewrite /fuel_map_le /fuel_map_le_inner map_included_spec in Hfmle.
@@ -891,7 +921,7 @@ Section model_state_lemmas.
       intros k v1 Hv2.
       rewrite /model_update_locale_role_map lookup_fmap in Hv2.
       apply fmap_Some in Hv2 as [? [Hv2 ->]].
-      pose proof Hv2 as Hv2'%map_lookup_filter_Some_1_2.
+      pose proof Hv2 as Hv2'%map_lookup_filter_Some_1_2. simpl in *.
       apply map_lookup_filter_Some_1_1 in Hv2.
       assert (k ∈ dom fs) as Hv2''.
       { destruct Hv2' as [Hv2'|Hv2']; [|done].
@@ -903,7 +933,7 @@ Section model_state_lemmas.
       rewrite -(dom_fmap_L S) in Hv2''.
       apply elem_of_dom in Hv2'' as [f Heq].
       pose proof Heq as Heq'.
-      apply lookup_fmap_Some in Heq' as [f' [<- _]].
+      apply lookup_fmap_Some in Heq' as [f' [<- ?]].
       apply Hle in Heq as [f'' [Heq Hle']].
       exists f''. split; [done|].
       destruct f''; [lia|].
@@ -946,7 +976,7 @@ Section model_state_lemmas.
     specialize (Hρs ρ (S f1) Hρ') as [v2 [Hv2 Hle]].
     destruct v2; [lia|]. exists v2. split; [|lia].
     rewrite !lookup_fmap map_lookup_filter Hv2=> /=.
-    destruct (decide (ρ ∈ live_roles M δ ∨ ρ ∈ dom fs)) as [Hin|Hnin].
+    destruct (decide (ρ ∈ usr_live_roles (usr_state δ) ∨ ρ ∈ dom fs)) as [Hin|Hnin].
     + rewrite option_guard_True; [|done]. simpl. f_equiv. lia.
     + apply Decidable.not_or in Hnin. destruct Hnin as [Hnin1 Hnin2].
       apply not_elem_of_dom in Hnin2. set_solver.
@@ -955,9 +985,9 @@ Section model_state_lemmas.
   Lemma fuel_map_preserve_dead_fuel_step fm ζ fs (δ:LM) :
     fm !! ζ = Some (S <$> fs) →
     fuel_map_preserve_dead fm
-      (M.(live_roles) $ model_update_locale_fuel δ ζ (dom fs)) →
+      (usr_live_roles $ usr_state $ model_update_locale_fuel δ ζ (dom fs)) →
     fuel_map_preserve_dead (<[ζ:=fs]> fm)
-      (M.(live_roles) $ (model_update_locale_fuel δ ζ (dom fs))).
+      (usr_live_roles $ usr_state $ (model_update_locale_fuel δ ζ (dom fs))).
   Proof.
     intros Hagree Hfmdead ρ Hin. apply Hfmdead in Hin as (ζ'&ρs&HSome&Hρ).
     destruct (decide (ζ = ζ')) as [<-|Hneq].
@@ -966,7 +996,7 @@ Section model_state_lemmas.
   Qed.
 
   Lemma fuel_map_preserve_threadpool_fuel_step
-        act c1 ζ c2 (fm1 fm2 : gmap _ (gmap (fmrole M) nat)) :
+        act c1 ζ c2 (fm1 fm2 : gmap _ (gmap (usr_role M) nat)) :
     dom fm1 = dom fm2 → locale_step c1 (inl (ζ, act)) c2 →
     fuel_map_preserve_threadpool c1.1 fm1 →
     fuel_map_preserve_threadpool c2.1 fm2.
@@ -988,10 +1018,10 @@ Section model_state_lemmas.
     has_fuels ζ fs.
   Proof.
     iIntros (Hstep) "Hm Hfs".
-    iDestruct "Hm" as "(?&%fm&[%Hfmle%Hdom]&%Hfmdead&%Htp&Hm&Hfm)".
+    iDestruct "Hm" as "(%fm&[%Hfmle%Hdom]&%Hfmdead&%Htp&Hm&Hfm)".
     iDestruct (has_fuels_agree with "Hfm Hfs") as %Hagree.
     iMod (has_fuels_decr with "Hfm Hfs") as "[Hfm $]".
-    iModIntro. iSplit; first iFrame. iExists _. iFrame. iPureIntro.
+    iModIntro. iExists _. iFrame. iPureIntro.
     split; [|split].
     - by apply fuel_map_le_fuel_step.
     - by apply fuel_map_preserve_dead_fuel_step.
@@ -1025,7 +1055,7 @@ Section model_state_lemmas.
   (** Model step *)
 
   (* OBS: Maybe use fuel limit instead of generic [f] *)
-  Program Definition model_update_set (ζ : locale Λ) (ρ : fmrole M) (f : nat) (δ : LM) : LM :=
+  Program Definition model_update_set (ζ : locale Λ) (ρ : usr_role M) (f : nat) (δ : LM) : LM :=
     {|
       ls_data :=
         {| ls_under := δ.(ls_under);
@@ -1057,13 +1087,13 @@ Section model_state_lemmas.
     - eexists ζ', _. by rewrite lookup_alter_ne.
   Qed.
 
-  Definition model_update_state (δ2 : M) (δ1 : LiveStateData Λ M) :
-    LiveStateData Λ M :=
+  Definition model_update_state (δ2 : joint_model M Net) (δ1 : LiveStateData Λ (joint_model M Net)) :
+    LiveStateData Λ _ :=
     {| ls_under := δ2;
       ls_map := δ1.(ls_map); |}.
 
-  Lemma model_update_state_valid (δ2 : M) (δ1 : LM) :
-    M.(live_roles) δ2 ⊆ M.(live_roles) δ1 →
+  Lemma model_update_state_valid (δ2 : joint_model M Net) (δ1 : LM) :
+    usr_live_roles δ2.1 ⊆ usr_live_roles (usr_state δ1) →
     ∃ δ, (ls_data δ) = model_update_state δ2 δ1.
   Proof.
     intros Hle.
@@ -1071,11 +1101,11 @@ Section model_state_lemmas.
               ζ ≠ ζ' → (model_update_state δ2 δ1).(ls_map) !! ζ = Some fs →
               (model_update_state δ2 δ1).(ls_map) !! ζ' = Some fs' → fs ##ₘ fs') as Hdisj'.
     { intros. by eapply (δ1.(ls_map_disj)). }
-    assert (∀ ρ, ρ ∈ M.(live_roles) (model_update_state δ2 δ1).(ls_under) →
+    assert (∀ ρ, ρ ∈ usr_live_roles $ usr_state (model_update_state δ2 δ1) →
                  ∃ ζ fs, (model_update_state δ2 δ1).(ls_map) !! ζ = Some fs ∧ ρ ∈ dom fs) as Hlive'.
     { pose proof (δ1.(ls_map_live)) as Hlive.
       intros.
-      assert (ρ ∈ live_roles M δ1) as Hin by set_solver.
+      assert (ρ ∈ usr_live_roles (usr_state δ1)) as Hin by set_solver.
       apply Hlive in Hin as (?&?&?&?). eexists _, _. done. }
     exists
       {| ls_data := model_update_state δ2 δ1;
@@ -1085,11 +1115,11 @@ Section model_state_lemmas.
   Qed.
 
   Definition model_update_model_step
-          (ζ : locale Λ) (ρs : gset (fmrole M)) ρ (δ2 : M) (δ : LM) : M :=
-    model_update_state δ2 $ model_update_set ζ ρ (LM.(lm_fl) δ2) $ model_update_decr ζ $ model_update_filter ζ ρs δ.
+          (ζ : locale Λ) (ρs : gset (usr_role M)) ρ δ2 (δ : LM) :=
+    model_update_state δ2 $ model_update_set ζ ρ (fm_fl δ2) $ model_update_decr ζ $ model_update_filter ζ ρs δ.
 
-  Lemma model_update_model_step_valid (ζ : locale Λ) (ρs : gset (fmrole M)) ρ (s2 : M) (δ1:LM) :
-    M.(live_roles) s2 ⊆ M.(live_roles) (ls_under δ1) →
+  Lemma model_update_model_step_valid (ζ : locale Λ) (ρs : gset (usr_role M)) ρ s2 (δ1:LM) :
+    usr_live_roles s2.1 ⊆ usr_live_roles (usr_state δ1) →
     ∃ δ, (ls_data δ) = model_update_model_step ζ ρs ρ s2 δ1.
   Proof. intros. by apply model_update_state_valid. Qed.
 
@@ -1110,29 +1140,29 @@ Section model_state_lemmas.
   Qed.
 
   (* OBS: Need to make frag model abstract *)
-  Lemma model_state_interp_model_step_update (ρ : fmrole M)
+  Lemma model_state_interp_model_step_update (ρ : usr_role M)
         fmact act
-        (fs : gmap (fmrole M) nat) tp1 tp2
-        (δ δ2 : LM) ζ σ1 σ2 (f1 : nat) s1 s2 :
+        (fs : gmap (usr_role M) nat) tp1 tp2
+        (δ δ2 : LM) ζ σ1 σ2 (f1 : nat) (s1 s2 : joint_model M Net) :
     ρ ∉ dom fs →
-    live_roles M s2 ⊆ live_roles M s1 →
+    usr_live_roles s2.1 ⊆ usr_live_roles s1.1 →
     locale_step (tp1, σ1) (inl (ζ, act)) (tp2, σ2) →
     fmtrans _ s1 (inl (ρ, fmact)) s2 →
     (ls_data δ2) = model_update_model_step ζ ({[ρ]} ∪ dom fs) ρ s2 δ →
     model_state_interp tp1 δ -∗
     has_fuels ζ ({[ρ := f1]} ∪ (S <$> fs)) -∗
-    frag_model_is s1 ==∗
+    frag_model_is s1.1 ==∗
     model_state_interp tp2 δ2 ∗
-    has_fuels ζ ({[ρ := LM.(lm_fl) s2]} ∪ fs) ∗
-    frag_model_is s2.
+    has_fuels ζ ({[ρ := fm_fl s2]} ∪ fs) ∗
+    frag_model_is s2.1.
   Proof.
     iIntros (Hfs Hlive Hstep Hmstep Hδ2) "Hm Hf Hs".
-    iDestruct "Hm" as "(?&%fm&%Hfmle&%Hfmdead&%Htp&Hm&Hfm)".
+    iDestruct "Hm" as "(%fm&%Hfmle&%Hfmdead&%Htp&Hm&Hfm)".
     iDestruct (has_fuels_agree with "Hfm Hf") as %Hagree.
-    iMod (has_fuels_update _ _ _ ({[ρ := lm_fl LM s2]} ∪ fs) with "Hfm Hf")
+    iMod (has_fuels_update _ _ _ ({[ρ := fm_fl s2]} ∪ fs) with "Hfm Hf")
       as "[Hfm Hf]".
-    iDestruct (model_agree with "Hm Hs") as %<-.
-    iMod (model_update _ _ s2 with "Hm Hs") as "[Hm Hs]".
+    iDestruct (model_agree with "Hm Hs") as %Heq.
+    iMod (model_update _ _ s2.1 with "Hm Hs") as "[Hm Hs]".
     iModIntro. iFrame. iExists _. iFrame.
     rewrite Hδ2. iFrame.
     iPureIntro.
@@ -1156,11 +1186,11 @@ Section model_state_lemmas.
       rewrite -(insert_id (ls_map δ) ζ fs'); [|done].
       rewrite !alter_insert.
       apply map_included_insert; [|done].
-      assert ({[ρ := lm_fl LM s2]} ∪ fs =
-              (alter (λ _ : nat, lm_fl LM s2) ρ
+      assert ({[ρ := usr_fl s2.1]} ∪ fs =
+              (alter (λ _ : nat, fm_fl s2) ρ
                      ((λ f : nat, f - 1) <$>
                                          (filter
-                                            (λ ρf : fmrole M * nat, ρf.1 ∈ live_roles M δ ∨ ρf.1 ∈ {[ρ]} ∪ dom fs)
+                                            (λ ρf : usr_role M * nat, ρf.1 ∈ usr_live_roles (usr_state δ) ∨ ρf.1 ∈ {[ρ]} ∪ dom fs)
                                             ({[ρ := f1]} ∪ (S <$> fs)))))) as ->.
       { rewrite -!insert_union_singleton_l.
         rewrite map_filter_insert. simpl.
@@ -1192,6 +1222,7 @@ Section model_state_lemmas.
     - apply elem_of_subseteq in Hlive.
       intros ρ' Hin.
       apply Hlive in Hin.
+      rewrite Heq in Hfmdead.
       apply Hfmdead in Hin as (ζ'&ρs&HSome&Hρ).
       destruct (decide (ζ = ζ')) as [<-|Hneq].
       + eexists ζ, _. rewrite lookup_insert. split; [done|]. by set_solver.
@@ -1209,23 +1240,23 @@ Section model_state_lemmas.
       set_solver.
   Qed.
 
-  Lemma model_step_suff_data_weak_alt (δ1 δ2 : LiveState Λ M) ρ fmact act
+  Lemma model_step_suff_data_weak_alt (δ1 δ2 : LiveState Λ (joint_model M Net)) ρ fmact act
         (fs fs': gmap _ nat) ζ :
     fmtrans _ δ1 (inl (ρ, fmact)) δ2 →
-    M.(live_roles) δ2 ⊆ M.(live_roles) δ1 →
+    usr_live_roles (usr_state δ2) ⊆ usr_live_roles (usr_state δ1) →
     δ1.(ls_map) !! ζ = Some fs →
     δ2.(ls_map) = <[ζ := fs']> δ1.(ls_map) →
     ρ ∈ dom fs →
-    fs' !! ρ = Some (LM.(lm_fl) (ls_under δ2)) →
+    fs' !! ρ = Some (fm_fl (ls_under δ2)) →
     map_included (<) (delete ρ fs') fs →
-    (dom fs ∖ dom fs' ∩ M.(live_roles) δ1 = ∅) →
-    ls_trans LM.(lm_fl) δ1 (Take_step ρ fmact ζ act) δ2.
+    (dom fs ∖ dom fs' ∩ usr_live_roles (usr_state δ1) = ∅) →
+    ls_trans fm_fl δ1 (Take_step ρ fmact ζ act) δ2.
   Proof.
     intros Hstep Hlive Hfs Hfs' Hρ Hρ' Hlt Hlive'.
-    assert (∃ (δ'':LiveState Λ M), δ''.(ls_data) =
+    assert (∃ (δ'': LiveState Λ _), δ''.(ls_data) =
           {| ls_under := ls_under δ2;
             ls_map := <[ζ := fs']> δ1.(ls_map) |} ∧
-            ls_trans LM.(lm_fl) δ1 (Take_step ρ fmact ζ act) δ'') as (δ''&Heq&Htrans).
+            ls_trans fm_fl δ1 (Take_step ρ fmact ζ act) δ'') as (δ''&Heq&Htrans).
     { eapply (model_step_suff_data); try done.
       - rewrite map_included_spec in Hlt.
         intros ρ' f f' Hf' Hneq Hf.
@@ -1238,38 +1269,44 @@ Section model_state_lemmas.
     rewrite Heq -Hfs' in Htrans. by destruct δ2, ls_data.
   Qed.
 
-  Definition model_can_model_step (δ1 : LM) (ζ : locale Λ) (ρ : fmrole M) (δ2 : LM) fmact : Prop :=
-    ∃ (fs fs' : gmap (fmrole M) nat),
+  Definition model_can_model_step (δ1 : LM) (ζ : locale Λ) (ρ : usr_role M) (δ2 : LM) fmact : Prop :=
+    ∃ (fs fs' : gmap (usr_role M) nat),
       fmtrans _ δ1 (inl (ρ, fmact)) δ2 ∧
-      M.(live_roles) δ2 ⊆ M.(live_roles) δ1 ∧
+      usr_live_roles (usr_state δ2) ⊆ usr_live_roles (usr_state δ1) ∧
       δ1.(ls_map) !! ζ = Some fs ∧
       δ2.(ls_map) = <[ζ := fs']> δ1.(ls_map) ∧
       ρ ∈ dom fs ∧
-      fs' !! ρ = Some (LM.(lm_fl) (ls_under δ2)) ∧
+      fs' !! ρ = Some (fm_fl (ls_under δ2)) ∧
       map_included (<) (delete ρ fs') fs ∧
-      (dom fs ∖ dom fs' ∩ M.(live_roles) δ1 = ∅).
+      (dom fs ∖ dom fs' ∩ usr_live_roles (usr_state δ1) = ∅).
 
-  Lemma model_can_model_step_trans ζ ρ (δ δ' : LiveState Λ M) fmact act:
-    model_can_model_step δ ζ ρ δ' fmact → ls_trans (LM.(lm_fl)) δ (Take_step ρ fmact ζ act) δ'.
+  Lemma model_can_model_step_trans ζ (ρ : fmrole (joint_model M Net))
+    (δ δ' : LiveState Λ (joint_model M Net)) fmact act:
+    model_can_model_step δ ζ ρ δ' fmact → ls_trans fm_fl δ (Take_step ρ fmact ζ act) δ'.
   Proof.
     destruct 1 as (?&?&?&?&?&?&?&?&?&?).
     by eapply model_step_suff_data_weak_alt.
   Qed.
 
   Lemma model_state_interp_can_model_step es (δ δ2 : LM) ζ ρ f fmact
-        (fs : gmap (fmrole M) nat) (s1 s2 : M) :
+        (fs : gmap (usr_role M) nat) (s1 s2 : joint_model M Net) :
     fmtrans _ s1 (inl (ρ, fmact)) s2 →
-    M.(live_roles) s2 ⊆ M.(live_roles) s1 →
+    usr_live_roles s2.1 ⊆ usr_live_roles s1.1 →
     ρ ∉ dom fs →
+    env_state δ = s1.2 →
     (ls_data δ2) = model_update_model_step ζ ({[ρ]} ∪ dom fs) ρ s2 δ →
     model_state_interp es δ -∗
     has_fuels ζ ({[ρ := f]} ∪ (S <$> fs)) -∗
-    frag_model_is s1 -∗
+    frag_model_is s1.1 -∗
     ⌜model_can_model_step δ ζ ρ δ2 fmact⌝.
   Proof.
-    iIntros (Hstep Hle Hρ Hδ2) "Hm Hf Hδ".
-    iDestruct "Hm" as "(?&%fm&%Hfmle&%Hfmdead&%Htp&Hm&Hfm)".
-    iDestruct (model_agree with "Hm Hδ") as %<-.
+    iIntros (Hstep Hle Hρ Henv Hδ2) "Hm Hf Hδ".
+    iDestruct "Hm" as "(%fm&%Hfmle&%Hfmdead&%Htp&Hm&Hfm)".
+    iDestruct (model_agree with "Hm Hδ") as %Heq.
+    have Heq': δ.(ls_under) = s1.
+    { destruct δ as [[[??] ?] ]. simpl in *.
+      rewrite /usr_state /= in Heq. rewrite /env_state /= in Henv.
+      rewrite Henv Heq. by destruct s1. }
     iDestruct (has_fuels_agree with "Hfm Hf") as %Hagree.
     iPureIntro.
     rewrite /fuel_map_le /fuel_map_le_inner map_included_spec in Hfmle.
@@ -1278,23 +1315,23 @@ Section model_state_lemmas.
     assert (ρ ∈ dom fs') as Hρ'.
     { apply map_included_subseteq_inv in Hfs'. set_solver. }
     eexists _, _. repeat split; try done.
-    - by rewrite Hδ2.
-    - by rewrite Hδ2.
+    - rewrite Hδ2 Heq' //.
+    - rewrite !Heq Hδ2 //.
     - rewrite Hδ2. simpl. rewrite -!alter_compose.
       rewrite -{1}(insert_id (ls_map δ) ζ fs'); [|done].
       rewrite alter_insert.
       f_equiv.
       done.
     - rewrite Hδ2. simpl. rewrite lookup_alter. rewrite lookup_fmap.
-      apply elem_of_dom in Hρ' as [f' Heq].
+      apply elem_of_dom in Hρ' as [f' Hlk].
       rewrite map_lookup_filter.
-      rewrite Heq. simpl.
+      rewrite Hlk. simpl.
       rewrite option_guard_True; [done|].
       set_solver.
     - rewrite map_included_spec.
       intros ρ' f' HSome.
       assert (ρ ≠ ρ').
-      { intros Heq. rewrite Heq in HSome.
+      { intros Heqρ. rewrite Heqρ in HSome.
         by rewrite lookup_delete in HSome. }
       rewrite lookup_delete_ne in HSome; [|done].
       exists (f' + 1).
@@ -1305,7 +1342,7 @@ Section model_state_lemmas.
       rewrite map_lookup_filter in HSome. simpl in *.
       destruct (fs' !! ρ') eqn:Heqn; [|done].
       simpl in *.
-      destruct (decide (ρ' ∈ live_roles M δ ∨ ρ' ∈ {[ρ]} ∪ dom fs)) as [Hin|Hnin].
+      destruct (decide (ρ' ∈ usr_live_roles (usr_state δ) ∨ ρ' ∈ {[ρ]} ∪ dom fs)) as [Hin|Hnin].
       + rewrite option_guard_True in HSome; [|done].
         simpl in *. simplify_eq. f_equiv.
         assert (ρ' ∈ dom ({[ρ := f]} ∪ (S <$> fs))) as Hin'.
@@ -1344,7 +1381,7 @@ Section model_state_lemmas.
   Qed.
 
   Lemma model_update_locale_spec_model_step extr
-        (auxtr : auxiliary_trace LM) ζ c2 ρs ρ δ2 s2 fmact act :
+        (auxtr : auxiliary_trace LM) ζ c2 ρs (ρ : fmrole (joint_model M Net)) δ2 s2 fmact act :
     (ls_data δ2) = model_update_model_step ζ ({[ρ]} ∪ ρs) ρ s2
                                            (trace_last auxtr) →
     model_can_model_step (trace_last auxtr) ζ ρ δ2 fmact →
@@ -1362,25 +1399,27 @@ Section model_state_lemmas.
 
   Lemma update_model_step
         (extr : execution_trace Λ)
-        (auxtr: auxiliary_trace LM) c2 (s1 s2 : M) fs ρ (δ1 : LM) ζ f fmact act :
-    M.(live_roles) s2 ⊆ M.(live_roles) s1 →
+        (auxtr: auxiliary_trace LM) c2 (s1 s2 : joint_model M Net) fs ρ (δ1 : LM) ζ f fmact act :
+    usr_live_roles s2.1 ⊆ usr_live_roles s1.1 →
     ρ ∉ dom fs →
     trace_last auxtr = δ1 →
     locale_step (trace_last extr) (inl (ζ, act)) c2 →
     fmtrans _ s1 (inl (ρ, fmact)) s2 →
-    has_fuels ζ ({[ρ := f]} ∪ (S <$> fs)) -∗ frag_model_is s1 -∗
+    env_state δ1 = s1.2 →
+    has_fuels ζ ({[ρ := f]} ∪ (S <$> fs)) -∗ frag_model_is s1.1 -∗
     ⌜valid_state_evolution_fairness extr auxtr⌝ -∗
     model_state_interp (trace_last extr).1 δ1 ==∗
     ∃ (δ2: LM),
       ⌜valid_state_evolution_fairness
         (extr :tr[inl (ζ, act)]: c2) (auxtr :tr[Take_step ρ fmact ζ act]: δ2)⌝ ∗
-      has_fuels ζ ({[ρ := LM.(lm_fl) s2]} ∪ fs) ∗
-      frag_model_is s2 ∗ model_state_interp c2.1 δ2.
+      has_fuels ζ ({[ρ := fm_fl s2]} ∪ fs) ∗
+      frag_model_is s2.1 ∗ model_state_interp c2.1 δ2.
   Proof.
-    iIntros (Hlive Hdom Hlast Hstep Htrans) "Hfuel Hfrag %Hvse Hm".
-    iDestruct (model_agree' with "Hm Hfrag") as %<-.
+    iIntros (Hlive Hdom Hlast Hstep Htrans Henv) "Hfuel Hfrag %Hvse Hm".
+    iDestruct (model_agree' with "Hm Hfrag") as %Heq.
     pose proof (model_update_model_step_valid
-                  ζ ({[ρ]} ∪ dom fs) ρ s2 δ1) as [δ2 Hδ2]; [done|].
+                  ζ ({[ρ]} ∪ dom fs) ρ s2 δ1) as [δ2 Hδ2].
+    { rewrite /usr_state Heq //. }
     iExists δ2.
     iDestruct (model_state_interp_can_model_step with "Hm Hfuel Hfrag")
       as %Hcan_step; [try done..|].
@@ -1400,14 +1439,14 @@ Section model_state_lemmas.
     ∃ tp1', tp2 = tp1' ++ [e] ∧ locales_equiv tp1 tp1'.
 
   Definition model_update_split
-             (ζ ζf : locale Λ) (ρs : gset (fmrole M))
-             (δ : LiveStateData Λ M) : LiveStateData Λ M :=
+             (ζ ζf : locale Λ) (ρs : gset (usr_role M))
+             (δ : LiveStateData Λ (joint_model M Net)) : LiveStateData Λ _ :=
     {| ls_under := δ.(ls_under);
        ls_map := <[ζf := (filter (λ ρf, ρf.1 ∈ ρs)) (δ.(ls_map) !!! ζ)]>
                    (alter (filter (λ ρf, ρf.1 ∉ ρs)) ζ δ.(ls_map)); |}.
 
-  Definition map_live (ρs : gset (fmrole M))
-             (m : gmap (locale Λ) (gmap (fmrole M) nat)) : Prop :=
+  Definition map_live (ρs : gset (usr_role M))
+             (m : gmap (locale Λ) (gmap (usr_role M) nat)) : Prop :=
     ∀ ρ, ρ ∈ ρs → ∃ ζ fs, m !! ζ = Some fs ∧ ρ ∈ dom fs.
 
   Lemma disjoint_subseteq `{Countable A} (xs1 xs2 ys1 ys2 : gset A) :
@@ -1448,7 +1487,7 @@ Section model_state_lemmas.
           rewrite HSome in HSome2. simpl in *. simplify_eq.
           apply map_disjoint_dom.
           pose proof (disjoint_filter_complement
-                        (λ ρ : fmrole M, ρ ∈ ρs) (dom ρs')) as Hcomp.
+                        (λ ρ : usr_role M, ρ ∈ ρs) (dom ρs')) as Hcomp.
           by rewrite !filter_dom_L in Hcomp. }
         rewrite lookup_alter_ne in HSome2; [|done].
         simplify_eq.
@@ -1468,7 +1507,7 @@ Section model_state_lemmas.
           simpl in *. simplify_eq.
           apply map_disjoint_dom.
           pose proof (disjoint_filter_complement
-                        (λ ρ : fmrole M, ρ ∈ ρs) (dom ρs')) as Hcomp.
+                        (λ ρ : usr_role M, ρ ∈ ρs) (dom ρs')) as Hcomp.
           by rewrite !filter_dom_L in Hcomp. }
         rewrite lookup_alter_ne in HSome1; [|done].
         rewrite lookup_total_alt in HSome2.
@@ -1506,7 +1545,7 @@ Section model_state_lemmas.
       rewrite lookup_alter_ne in HSome2; [|done].
       pose proof (Hdisj ζ1 ζ2 _ _ Hneq' HSome1 HSome2).
       done. }
-    assert (map_live (M.(live_roles) δ2) δ2.(ls_map)) as Hlive.
+    assert (map_live (usr_live_roles (usr_state δ2)) δ2.(ls_map)) as Hlive.
     { intros ρ Hin.
       pose proof (δ1.(ls_map_live)) as Hlive.
       apply Hlive in Hin as (ζ'&fs&HSome'&Hin').
@@ -1516,13 +1555,13 @@ Section model_state_lemmas.
       { rewrite HSome in HSome'. simplify_eq.
         simpl.
         destruct (decide (ρ ∈ ρs)) as [Hin|Hnin'].
-        - exists ζf, (filter (λ ρf : fmrole M * nat, ρf.1 ∈ ρs) fs).
+        - exists ζf, (filter (λ ρf : usr_role M * nat, ρf.1 ∈ ρs) fs).
           rewrite lookup_insert. rewrite lookup_total_alt. rewrite HSome. simpl.
           split; [done|].
           apply elem_of_dom. rewrite /is_Some.
           apply elem_of_dom in Hin' as [??].
           eexists _. by apply map_lookup_filter_Some_2.
-        - exists ζ, (filter (λ ρf : fmrole M * nat, ρf.1 ∉ ρs) fs).
+        - exists ζ, (filter (λ ρf : usr_role M * nat, ρf.1 ∉ ρs) fs).
           rewrite lookup_insert_ne; [|done].
           rewrite lookup_alter. rewrite HSome. simpl.
           split; [done|].
@@ -1541,14 +1580,14 @@ Section model_state_lemmas.
 
   Definition model_update_fork
           (ζ : locale Λ) (ζf : locale Λ)
-          (ρs1 ρs2 : gset (fmrole M)) (δ : LM) :
-      LiveStateData Λ M :=
+          (ρs1 ρs2 : gset (usr_role M)) (δ : LM) :
+      LiveStateData Λ _ :=
     model_update_split ζ ζf ρs2 $
     model_update_decr ζ $
     model_update_filter ζ ρs1 δ.
 
   Lemma model_update_fork_valid
-        ζ ζf (ρs1 ρs2 : gset (fmrole M)) (δ1 : LM) :
+        ζ ζf (ρs1 ρs2 : gset (usr_role M)) (δ1 : LM) :
     ζ ∈ dom δ1.(ls_map) → ζf ∉ dom δ1.(ls_map) →
     ∃ δ2, (ls_data δ2) = model_update_fork ζ ζf ρs1 ρs2 δ1.
   Proof. intros ??. by apply model_update_split_valid; set_solver. Qed.
@@ -1588,7 +1627,7 @@ Section model_state_lemmas.
     unfold locales_of_list_from.
     intros Habs.
     apply elem_of_list_fmap in Habs as ((tp1&e1) & Hlo & Hpf).
-    apply prefixes_from_spec in Hpf as (tp2&tp3&He1&He2).
+    apply (prefixes_from_spec [] tp e1 tp1) in Hpf as (tp2&tp3&He1&He2).
     simplify_eq.
     list_simplifier.
 
@@ -1619,7 +1658,7 @@ Section model_state_lemmas.
     has_fuels (locale_of tp1 efork) fs2.
   Proof.
     iIntros (Hδ2 Hfs Hdisj Hforked Hstep) "Hm Hf".
-    iDestruct "Hm" as "(?&%fm&%Hfmle&%Hfmdead&%Htp&Hm&Hfm)".
+    iDestruct "Hm" as "(%fm&%Hfmle&%Hfmdead&%Htp&Hm&Hfm)".
     iDestruct (has_fuels_agree with "Hfm Hf") as %Hagree.
     assert (locale_of tp1 efork ∉ dom fm) as Hnin.
     { pose proof (not_elem_of_locale_of_from_list tp1 efork) as Hes%Htp.
@@ -1691,8 +1730,7 @@ Section model_state_lemmas.
           eapply disjoint_subseteq_r; [apply dom_filter_subseteq|].
           set_solver. }
         rewrite map_filter_id; last first.
-        { simpl.
-          intros. apply elem_of_dom_2 in H0.
+        { simpl. intros ? ? Hlk. apply elem_of_dom_2 in Hlk.
           apply map_agree_R_dom in Hfs1'.
           apply map_agree_R_dom in Hfs2'.
           split; [set_solver|].
@@ -1721,11 +1759,10 @@ Section model_state_lemmas.
       { apply map_union_subseteq_l. }
 
       rewrite map_filter_id; last first.
-      { simpl.
-        intros. apply elem_of_dom_2 in H0.
+      { simpl. intros ?? Hlk. apply elem_of_dom_2 in Hlk.
         apply map_agree_R_dom in Hfs1'.
         apply map_agree_R_dom in Hfs2'.
-        rewrite dom_fmap in H0.
+        rewrite dom_fmap in Hlk.
         apply map_disjoint_dom in Hdisj.
         split; [set_solver|].
         set_solver. }
@@ -1778,17 +1815,17 @@ Section model_state_lemmas.
       δ2.(ls_map) = <[ζ := fs1]>(<[ζf := fs2]> δ1.(ls_map)) ∧
       map_included (<) fs1 fs ∧
       map_included (<) fs2 fs ∧
-      (dom fs ∖ (dom fs1 ∪ dom fs2) ∩ M.(live_roles) δ1 = ∅) ∧
+      (dom fs ∖ (dom fs1 ∪ dom fs2) ∩ usr_live_roles (usr_state δ1) = ∅) ∧
       (dom fs1 ∩ dom fs2 = ∅) ∧
       ζf ∉ dom δ1.(ls_map).
 
-  Lemma silent_step_suff_data_fork_weak act fl `(δ: LiveState Λ M)
+  Lemma silent_step_suff_data_fork_weak act fl `(δ: LiveState Λ (joint_model M Net))
         (fs fs1 fs2 : gmap _ nat) ζ ζf :
     δ.(ls_map) !! ζ = Some fs →
     fs ≠ ∅ →
     map_included (<) fs1 fs →
     map_included (<) fs2 fs →
-    (dom fs ∖ (dom fs1 ∪ dom fs2)) ∩ M.(live_roles) δ = ∅ →
+    (dom fs ∖ (dom fs1 ∪ dom fs2)) ∩ usr_live_roles (usr_state δ) = ∅ →
     (dom fs1 ∩ dom fs2 = ∅) →
     ζf ∉ dom δ.(ls_map) →
     ∃ δ', δ'.(ls_data) =
@@ -1796,15 +1833,15 @@ Section model_state_lemmas.
             ls_map := <[ζ := fs1]>(<[ζf := fs2]> δ.(ls_map)) |} ∧
             ls_trans fl δ (Silent_step ζ act) δ'.
   Proof.
-    intros.
+    intros ?? Hincl1 Hincl2 **.
     apply (silent_step_suff_data fl δ fs fs1 fs2 ζ (Some ζf)); try done.
-    - rewrite map_included_spec in H2. done.
-    - rewrite map_included_spec in H3. done.
+    - rewrite map_included_spec in Hincl1. done.
+    - rewrite map_included_spec in Hincl2. done.
     - set_solver.
   Qed.
 
   (* TODO: Change original lemma to not existentially quantify new state *)
-  Lemma silent_step_suff_data_fork_weak_alt act fl (δ δ': LiveState Λ M)
+  Lemma silent_step_suff_data_fork_weak_alt act fl (δ δ': LiveState Λ (joint_model M Net))
         (fs fs1 fs2 : gmap _ nat) ζ ζf :
     δ.(ls_under) = δ'.(ls_under) →
     δ.(ls_map) !! ζ = Some fs →
@@ -1812,7 +1849,7 @@ Section model_state_lemmas.
     fs ≠ ∅ →
     map_included (<) fs1 fs →
     map_included (<) fs2 fs →
-    (dom fs ∖ (dom fs1 ∪ dom fs2)) ∩ M.(live_roles) δ = ∅ →
+    (dom fs ∖ (dom fs1 ∪ dom fs2)) ∩ usr_live_roles (usr_state δ) = ∅ →
     (dom fs1 ∩ dom fs2 = ∅) →
     ζf ∉ dom δ.(ls_map) →
     ls_trans fl δ (Silent_step ζ act) δ'.
@@ -1828,7 +1865,7 @@ Section model_state_lemmas.
     rewrite Heq Hδ -Hfs12 in Htrans. by destruct δ', ls_data.
   Qed.
 
-  Lemma model_can_fork_step_trans act fl ζ ζf (δ δ' : LiveState Λ M) :
+  Lemma model_can_fork_step_trans act fl ζ ζf (δ δ' : LiveState Λ (joint_model M Net)) :
     model_can_fork_step δ ζ ζf δ' → ls_trans fl δ (Silent_step ζ act) δ'.
   Proof.
     destruct 1 as (?&?&?&?&?&?&?&?&?&?&?&?).
@@ -1836,14 +1873,14 @@ Section model_state_lemmas.
   Qed.
 
   Lemma model_state_interp_can_fork_step es (δ1 δ2 : LM) ζ
-        (fs1 fs2 : gmap (fmrole M) nat) e :
+        (fs1 fs2 : gmap (usr_role M) nat) e :
     (ls_data δ2) = model_update_fork ζ (locale_of es e) (dom fs1 ∪ dom fs2) (dom fs2) δ1 →
     (fs1 ∪ fs2) ≠ ∅ → fs1 ##ₘ fs2 →
     model_state_interp es δ1 -∗ has_fuels_S ζ (fs1 ∪ fs2) -∗
     ⌜model_can_fork_step δ1 ζ (locale_of es e) δ2⌝.
   Proof.
     iIntros (Hδ2 Hne Hdisj) "Hm Hf".
-    iDestruct "Hm" as "(?&%fm&[%Hfmle %Hdom]&%Hfmdead&%Htp&Hm&Hfm)".
+    iDestruct "Hm" as "(%fm&[%Hfmle %Hdom]&%Hfmdead&%Htp&Hm&Hfm)".
     iDestruct (has_fuels_agree with "Hfm Hf") as %Hagree.
     pose proof Hagree as Hagree'.
     rewrite /fuel_map_le_inner map_included_spec in Hfmle.
@@ -1887,7 +1924,7 @@ Section model_state_lemmas.
         rewrite map_filter_union; [|apply map_disjoint_dom; set_solver].
         assert (filter
                   (λ '(i, _),
-                     i ∈ dom fs2 ∧ (i ∈ live_roles M δ1 ∨ i ∈ dom fs1 ∪ dom fs2))
+                     i ∈ dom fs2 ∧ (i ∈ usr_live_roles (usr_state δ1) ∨ i ∈ dom fs1 ∪ dom fs2))
                   (S <$> fs1') = ∅) as Hfs1'.
         { apply map_filter_empty_iff.
           intros ρ f Hρ [HP1 HP2].
@@ -1895,7 +1932,7 @@ Section model_state_lemmas.
           rewrite dom_fmap_L in Hρ. set_solver. }
         assert (filter
                   (λ '(i, _),
-                     i ∈ dom fs2 ∧ (i ∈ live_roles M δ1 ∨ i ∈ dom fs1 ∪ dom fs2))
+                     i ∈ dom fs2 ∧ (i ∈ usr_live_roles (usr_state δ1) ∨ i ∈ dom fs1 ∪ dom fs2))
                   fsf' = ∅) as Hfsf'.
         { apply map_filter_empty_iff.
           intros ρ f Hρ [HP1 HP2].
@@ -1903,10 +1940,10 @@ Section model_state_lemmas.
         rewrite Hfs1' Hfsf'.
         rewrite left_id right_id.
         rewrite map_filter_id; last first.
-        { intros. split.
-          - apply elem_of_dom_2 in H0. set_solver.
+        { intros ?? Hlk. split.
+          - apply elem_of_dom_2 in Hlk. set_solver.
           - right.
-            apply elem_of_dom_2 in H0. set_solver. }
+            apply elem_of_dom_2 in Hlk. set_solver. }
         rewrite -map_fmap_compose.
         rewrite decr_succ_compose_id.
         rewrite map_fmap_id.
@@ -1926,7 +1963,7 @@ Section model_state_lemmas.
       rewrite map_filter_union; [|apply map_disjoint_dom; set_solver].
       assert (filter
              (λ '(i, _),
-                (i ∉ dom fs2) ∧ (i ∈ live_roles M δ1 ∨ i ∈ dom fs1 ∪ dom fs2))
+                (i ∉ dom fs2) ∧ (i ∈ usr_live_roles (usr_state δ1) ∨ i ∈ dom fs1 ∪ dom fs2))
              (S <$> fs2') = ∅) as Hfs2'.
       { apply map_filter_empty_iff.
         intros ρ f Hρ [HP1 HP2].
@@ -1934,7 +1971,7 @@ Section model_state_lemmas.
         rewrite dom_fmap_L in Hρ. set_solver. }
       assert (filter
                 (λ '(i, _),
-                   (i ∉ dom fs2) ∧ (i ∈ live_roles M δ1 ∨ i ∈ dom fs1 ∪ dom fs2))
+                   (i ∉ dom fs2) ∧ (i ∈ usr_live_roles (usr_state δ1) ∨ i ∈ dom fs1 ∪ dom fs2))
                 fsf' = ∅) as Hfsf'.
       { apply map_filter_empty_iff.
         intros ρ f Hρ [HP1 HP2].
@@ -1958,10 +1995,10 @@ Section model_state_lemmas.
       rewrite Hfs2' Hfsf'.
       rewrite right_id right_id.
       rewrite map_filter_id; last first.
-      { intros. split.
-        - apply elem_of_dom_2 in H0. set_solver.
+      { intros ?? Hlk. split.
+        - apply elem_of_dom_2 in Hlk. set_solver.
         - right.
-          apply elem_of_dom_2 in H0. set_solver. }
+          apply elem_of_dom_2 in Hlk. set_solver. }
       rewrite -map_fmap_compose.
       rewrite decr_succ_compose_id.
       rewrite map_fmap_id.
@@ -2034,12 +2071,12 @@ Section model_state_lemmas.
     econstructor=>//; first by eapply model_can_fork_step_trans.
   Qed.
 
-  Lemma model_state_interp_has_fuels_agree es δ ζ (fs : gmap (fmrole M) nat) :
+  Lemma model_state_interp_has_fuels_agree es δ ζ (fs : gmap (usr_role M) nat) :
     model_state_interp es δ -∗ has_fuels ζ fs -∗
     ⌜∃ fs', δ.(ls_map) !! ζ = Some fs' ∧ map_included (≤) fs fs'⌝.
   Proof.
     iIntros "Hm Hf".
-    iDestruct "Hm" as "(?&%fm&[%Hfmle %Hdom]&%Hfmdead&%Htp&Hm&Hfm)".
+    iDestruct "Hm" as "(%fm&[%Hfmle %Hdom]&%Hfmdead&%Htp&Hm&Hfm)".
     iDestruct (has_fuels_agree with "Hfm Hf") as %Hagree.
     rewrite /fuel_map_le_inner map_included_spec in Hfmle.
     apply Hfmle in Hagree as (fs'&HSome&Hfs').
@@ -2066,7 +2103,7 @@ Section model_state_lemmas.
       as %(fs'&HSome&Hfs').
     iAssert (⌜(locale_of tp1 efork) ∉ dom (ls_map (trace_last auxtr))⌝)%I as %Hnin.
     { destruct Hforked as (?&?&?).
-      iDestruct "Hm" as "(?&%fm&[%Hfmle %Hdom']&%Hfmdead&%Htp&Hm&Hfm)".
+      iDestruct "Hm" as "(%fm&[%Hfmle %Hdom']&%Hfmdead&%Htp&Hm&Hfm)".
       rewrite -Hdom'.
       iPureIntro. apply not_elem_of_dom. apply Htp.
       apply locale_step_equiv in Hstep. simpl in *.
